Cleaned up records

Lambda.thy
@@ -12,14 +12,6 @@ fun lookup :: "nat \<Rightarrow> 'a list \<Rightarrow> 'a option" where
 | "lookup 0 (a # as) = Some a"
 | "lookup (Suc x) (a # as) = lookup x as"
 
-fun lookup_assoc :: "'k \<Rightarrow> ('k \<times> 'v) list \<Rightarrow> 'v option" where
-  "lookup_assoc k [] = None"
-| "lookup_assoc k ((k', v) # as) = (if k = k' then Some v else lookup_assoc k as)"
-
-fun keys :: "('k \<times> 'v) list \<Rightarrow> 'k set" where
-  "keys [] = {}"
-| "keys ((k, v) # as) = insert k (keys as)"
-
 lemma [simp]: "x \<le> length as \<Longrightarrow> length (insert_at x a as) = Suc (length as)"
   by (induction x a as rule: insert_at.induct) simp_all
 
@@ -38,68 +30,55 @@ lemma [simp]: "x \<le> length as \<Longrightarrow> x \<le> y \<Longrightarrow> l
     thus ?case by (induction y) simp_all
   qed simp_all
 
-lemma [simp]: "keys (as @ bs) = keys as \<union> keys bs"
-  by (induction as rule: keys.induct) simp_all
-
 (* syntax *)
-
-typedecl label
 
 datatype type = 
   Base
 | Arrow type type
-| Record "(label \<times> type) list"
+| Record "type list"
 
 datatype expr = 
   Var nat
 | Abs type expr
 | App expr expr
-| Rec "(label \<times> expr) list"
-| Proj expr label
+| Rec "expr list"
+| Proj expr nat
 
-fun incr :: "nat \<Rightarrow> expr \<Rightarrow> expr"
-and incr_fs :: "nat \<Rightarrow> (label \<times> expr) list \<Rightarrow> (label \<times> expr) list" where
+primrec incr :: "nat \<Rightarrow> expr \<Rightarrow> expr" where
   "incr x (Var y) = Var (if x \<le> y then Suc y else y)"
 | "incr x (Abs t e) = Abs t (incr (Suc x) e)"
 | "incr x (App e\<^sub>1 e\<^sub>2) = App (incr x e\<^sub>1) (incr x e\<^sub>2)"
-| "incr x (Rec fs) = Rec (incr_fs x fs)"
+| "incr x (Rec fs) = Rec (map (incr x) fs)"
 | "incr x (Proj e l) = Proj (incr x e) l"
-| "incr_fs x [] = []"
-| "incr_fs x ((l, e) # fs) = (l, incr x e) # incr_fs x fs"
 
-fun subst :: "nat \<Rightarrow> expr \<Rightarrow> expr \<Rightarrow> expr" 
-and subst_fs :: "nat \<Rightarrow> expr \<Rightarrow> (label \<times> expr) list \<Rightarrow> (label \<times> expr) list" where
+primrec subst :: "nat \<Rightarrow> expr \<Rightarrow> expr \<Rightarrow> expr" where
   "subst x e' (Var y) = (if x = y then e' else Var (if x < y then y - 1 else y))"
 | "subst x e' (Abs t e) = Abs t (subst (Suc x) (incr 0 e') e)"
 | "subst x e' (App e\<^sub>1 e\<^sub>2) = App (subst x e' e\<^sub>1) (subst x e' e\<^sub>2)"
-| "subst x e' (Rec fs) = Rec (subst_fs x e' fs)"
+| "subst x e' (Rec fs) = Rec (map (subst x e') fs)"
 | "subst x e' (Proj e l) = Proj (subst x e' e) l"
-| "subst_fs x e' [] = []"
-| "subst_fs x e' ((l, e) # fs) = (l, subst x e' e) # subst_fs x e' fs"
 
-fun is_value :: "expr \<Rightarrow> bool" 
-and is_value_f :: "(label \<times> expr) list \<Rightarrow> bool" where
+primrec is_value :: "expr \<Rightarrow> bool" 
+    and is_value_f :: "expr list \<Rightarrow> bool" where
   "is_value (Var y) = False"
 | "is_value (Abs t e) = True"
 | "is_value (App e\<^sub>1 e\<^sub>2) = False"
 | "is_value (Rec fs) = is_value_f fs"
 | "is_value (Proj e l) = False"
 | "is_value_f [] = True"
-| "is_value_f ((l, e) # fs) = (is_value e \<and> is_value_f fs)"
+| "is_value_f (e # fs) = (is_value e \<and> is_value_f fs)"
 
 (* typechecking *)
 
 inductive typecheck :: "type list \<Rightarrow> expr \<Rightarrow> type \<Rightarrow> bool" (infix "\<turnstile> _ :" 60) 
-      and typecheck_fs :: "type list \<Rightarrow> (label \<times> expr) list \<Rightarrow> (label \<times> type) list \<Rightarrow> bool" 
-        (infix "\<turnstile>\<^sub>f _ :" 60) where
+      and typecheck_fs :: "type list \<Rightarrow> expr list \<Rightarrow> type list \<Rightarrow> bool" (infix "\<turnstile>\<^sub>f _ :" 60) where
   tc_var [simp]: "lookup x \<Gamma> = Some t \<Longrightarrow> \<Gamma> \<turnstile> Var x : t"
 | tc_abs [simp]: "t\<^sub>1 # \<Gamma> \<turnstile> e : t\<^sub>2 \<Longrightarrow> \<Gamma> \<turnstile> Abs t\<^sub>1 e : Arrow t\<^sub>1 t\<^sub>2"
 | tc_app [simp]: "\<Gamma> \<turnstile> e\<^sub>1 : Arrow t\<^sub>1 t\<^sub>2 \<Longrightarrow> \<Gamma> \<turnstile> e\<^sub>2 : t\<^sub>1 \<Longrightarrow> \<Gamma> \<turnstile> App e\<^sub>1 e\<^sub>2 : t\<^sub>2"
 | tc_rec [simp]: "\<Gamma> \<turnstile>\<^sub>f fs : ts \<Longrightarrow> \<Gamma> \<turnstile> Rec fs : Record ts"
-| tc_proj [simp]: "\<Gamma> \<turnstile> e : Record ts \<Longrightarrow> lookup_assoc l ts = Some t \<Longrightarrow> \<Gamma> \<turnstile> Proj e l : t"
+| tc_proj [simp]: "\<Gamma> \<turnstile> e : Record ts \<Longrightarrow> lookup l ts = Some t \<Longrightarrow> \<Gamma> \<turnstile> Proj e l : t"
 | tcf_nil [simp]: "\<Gamma> \<turnstile>\<^sub>f [] : []"
-| tcf_cons [simp]: "\<Gamma> \<turnstile> e : t \<Longrightarrow> \<Gamma> \<turnstile>\<^sub>f fs : ts \<Longrightarrow> l \<notin> keys fs \<Longrightarrow> 
-    \<Gamma> \<turnstile>\<^sub>f (l, e) # fs : (l, t) # ts"
+| tcf_cons [simp]: "\<Gamma> \<turnstile> e : t \<Longrightarrow> \<Gamma> \<turnstile>\<^sub>f fs : ts \<Longrightarrow> \<Gamma> \<turnstile>\<^sub>f e # fs : t # ts"
 
 inductive_cases [elim]: "\<Gamma> \<turnstile> Var x : t"
 inductive_cases [elim]: "\<Gamma> \<turnstile> Abs t\<^sub>1 e : t"
@@ -107,15 +86,15 @@ inductive_cases [elim]: "\<Gamma> \<turnstile> App e\<^sub>1 e\<^sub>2 : t"
 inductive_cases [elim]: "\<Gamma> \<turnstile> Rec fs : t"
 inductive_cases [elim]: "\<Gamma> \<turnstile> Proj e l : t"
 inductive_cases [elim]: "\<Gamma> \<turnstile>\<^sub>f [] : ts"
-inductive_cases [elim]: "\<Gamma> \<turnstile>\<^sub>f (l, e) # fs : ts"
+inductive_cases [elim]: "\<Gamma> \<turnstile>\<^sub>f e # fs : ts"
 
 (* evaluation *)
 
 datatype stack = 
   SApp1 expr
 | SApp2 expr
-| SRec "(label \<times> expr) list" label "(label \<times> expr) list" 
-| SProj label
+| SRec "expr list" "expr list" 
+| SProj nat
 
 inductive typecheck_stack :: "type list \<Rightarrow> stack list \<Rightarrow> type \<Rightarrow> type \<Rightarrow> bool" 
     (infix "\<turnstile> _ : _ \<rightarrow>" 60) where
@@ -123,17 +102,15 @@ inductive typecheck_stack :: "type list \<Rightarrow> stack list \<Rightarrow> t
 | tc_sapp1 [simp]: "\<Gamma> \<turnstile> s : t \<rightarrow> Arrow t\<^sub>1 t\<^sub>2 \<Longrightarrow> \<Gamma> \<turnstile> e : t\<^sub>1 \<Longrightarrow> \<Gamma> \<turnstile> SApp1 e # s : t \<rightarrow> t\<^sub>2"
 | tc_sapp2 [simp]: "\<Gamma> \<turnstile> e : Arrow t\<^sub>1 t\<^sub>2 \<Longrightarrow> \<Gamma> \<turnstile> s : t \<rightarrow> t\<^sub>1 \<Longrightarrow> \<Gamma> \<turnstile> SApp2 e # s : t \<rightarrow> t\<^sub>2"
 | tc_srec [simp]: "\<Gamma> \<turnstile>\<^sub>f vs : vts \<Longrightarrow> \<Gamma> \<turnstile>\<^sub>f nvs : nvts \<Longrightarrow> \<Gamma> \<turnstile> s : t \<rightarrow> t' \<Longrightarrow> 
-    keys vs \<inter> keys nvs = {} \<Longrightarrow> l \<notin> keys vs \<Longrightarrow> l \<notin> keys nvs \<Longrightarrow> 
-      \<Gamma> \<turnstile> SRec vs l nvs # s : t \<rightarrow> Record (vts @ [(l, t')] @ nvts)"
-| tc_sproj [simp]: "\<Gamma> \<turnstile> s : t \<rightarrow> Record ts \<Longrightarrow> lookup_assoc l ts = Some t' \<Longrightarrow> 
+    \<Gamma> \<turnstile> SRec vs nvs # s : t \<rightarrow> Record (vts @ [t'] @ nvts)"
+| tc_sproj [simp]: "\<Gamma> \<turnstile> s : t \<rightarrow> Record ts \<Longrightarrow> lookup l ts = Some t' \<Longrightarrow> 
     \<Gamma> \<turnstile> SProj l # s : t \<rightarrow> t'"
 
 fun stack_extend :: "stack \<Rightarrow> stack list \<times> expr \<Rightarrow> stack list \<times> expr" where
   "stack_extend s' se = (case se of (s, e) \<Rightarrow> (s' # s, e))"
 
 fun unfold :: "expr \<Rightarrow> stack list \<times> expr" 
-and unfold_f :: "(label \<times> expr) list \<Rightarrow> 
-      (label \<times> expr) list \<times> label \<times> (label \<times> expr) list \<times> stack list \<times> expr" where
+and unfold_f :: "expr list \<Rightarrow> expr list \<times> expr list \<times> stack list \<times> expr" where
   "unfold (Var y) = ([], Var y)"
 | "unfold (Abs t e) = ([], Abs t e)"
 | "unfold (App e\<^sub>1 e\<^sub>2) = (
@@ -145,27 +122,27 @@ and unfold_f :: "(label \<times> expr) list \<Rightarrow>
 | "unfold (Rec fs) = (
     if is_value_f fs 
     then ([], Rec fs) 
-    else case unfold_f fs of (vs, l, nvs, s, e) \<Rightarrow> (SRec vs l nvs # s, e))"
+    else case unfold_f fs of (vs, nvs, s, e) \<Rightarrow> (SRec vs nvs # s, e))"
 | "unfold (Proj e l) = (
     if is_value e 
     then ([], Proj e l) 
     else stack_extend (SProj l) (unfold e))"
 | "unfold_f [] = undefined"
-| "unfold_f ((l, e) # fs) = (
+| "unfold_f (e # fs) = (
     if is_value e
-    then case unfold_f fs of (vs, l', nvs, s, e') \<Rightarrow> ((l, e) # vs, l', nvs, s, e')
-    else ([], l, fs, unfold e))"
+    then case unfold_f fs of (vs, nvs, s, e') \<Rightarrow> (e # vs, nvs, s, e')
+    else ([], fs, unfold e))"
 
 fun fold :: "stack list \<Rightarrow> expr \<Rightarrow> expr" where
   "fold [] e = e"
 | "fold (SApp1 e' # s) e = App (fold s e) e'"
 | "fold (SApp2 e' # s) e = App e' (fold s e)"
-| "fold (SRec vs l nvs # s) e = Rec (vs @ [(l, fold s e)] @ nvs)"
+| "fold (SRec vs nvs # s) e = Rec (vs @ [fold s e] @ nvs)"
 | "fold (SProj l # s) e = Proj (fold s e) l"
 
 inductive reduce :: "expr \<Rightarrow> expr \<Rightarrow> bool" (infix "\<leadsto>\<^sub>\<beta>" 60) where
   ev_beta [simp]: "is_value e\<^sub>2 \<Longrightarrow> App (Abs t e\<^sub>1) e\<^sub>2 \<leadsto>\<^sub>\<beta> subst 0 e\<^sub>2 e\<^sub>1" 
-| ev_proj [simp]: "is_value_f fs \<Longrightarrow> lookup_assoc l fs = Some e \<Longrightarrow> Proj (Rec fs) l \<leadsto>\<^sub>\<beta> e" 
+| ev_proj [simp]: "is_value_f fs \<Longrightarrow> lookup l fs = Some e \<Longrightarrow> Proj (Rec fs) l \<leadsto>\<^sub>\<beta> e" 
 
 inductive evaluate :: "expr \<Rightarrow> expr \<Rightarrow> bool" (infix "\<leadsto>" 60) where
   ev_stack [simp]: "unfold e = (s, r) \<Longrightarrow> r \<leadsto>\<^sub>\<beta> r' \<Longrightarrow> e \<leadsto> fold s r'"
@@ -175,9 +152,9 @@ inductive_cases [elim]: "e \<leadsto> e'"
 (* safety *)
 
 lemma [simp]: "unfold e = (s, e') \<Longrightarrow> fold s e' = e"
-  and [simp]: "unfold_f fs = (vs, l, nvs, s, e') \<Longrightarrow> \<not> is_value_f fs \<Longrightarrow> 
-    vs @ [(l, fold s e')] @ nvs = fs"
-  by (induction e and fs arbitrary: s e' and vs l nvs s e' rule: unfold_unfold_f.induct) 
+  and [simp]: "unfold_f fs = (vs,  nvs, s, e') \<Longrightarrow> \<not> is_value_f fs \<Longrightarrow> 
+    vs @ [fold s e'] @ nvs = fs"
+  by (induction e and fs arbitrary: s e' and vs nvs s e' rule: unfold_unfold_f.induct) 
      (auto split: if_splits prod.splits)
 
 lemma canonical_arrow [simp]: "\<Gamma> \<turnstile> e : Arrow t\<^sub>1 t\<^sub>2 \<Longrightarrow> is_value e \<Longrightarrow> \<exists>e'. e = Abs t\<^sub>1 e'"
@@ -187,12 +164,12 @@ lemma canonical_record [simp]: "\<Gamma> \<turnstile> e : Record ts \<Longrighta
     \<exists>fs. e = Rec fs \<and> is_value_f fs \<and> \<Gamma> \<turnstile>\<^sub>f fs : ts"
   by (induction \<Gamma> e "Record ts" rule: typecheck_typecheck_fs.inducts(1)) simp_all
 
-lemma [simp]: "\<Gamma> \<turnstile>\<^sub>f fs : ts \<Longrightarrow> lookup_assoc l ts = Some t \<Longrightarrow> \<exists>e. lookup_assoc l fs = Some e"
-  by (induction \<Gamma> fs ts rule: typecheck_typecheck_fs.inducts(2)) (simp, simp_all split: if_splits)
+lemma [simp]: "\<Gamma> \<turnstile>\<^sub>f fs : ts \<Longrightarrow> lookup l ts = Some t \<Longrightarrow> \<exists>e. lookup l fs = Some e"
+  by (induction l fs arbitrary: ts rule: lookup.induct) auto
 
 theorem progress: "[] \<turnstile> e : t \<Longrightarrow> is_value e \<or> (\<exists>e'. e \<leadsto> e')"
-    and "[] \<turnstile>\<^sub>f fs : ts \<Longrightarrow> \<not> is_value_f fs \<Longrightarrow> unfold_f fs = (vs, lr, nvs, s, r) \<Longrightarrow> \<exists>r'. r \<leadsto>\<^sub>\<beta> r'"
-  proof (induction "[] :: type list" e t and "[] :: type list" fs ts arbitrary: and vs lr nvs s r 
+    and "[] \<turnstile>\<^sub>f fs : ts \<Longrightarrow> \<not> is_value_f fs \<Longrightarrow> unfold_f fs = (vs, nvs, s, r) \<Longrightarrow> \<exists>r'. r \<leadsto>\<^sub>\<beta> r'"
+  proof (induction "[] :: type list" e t and "[] :: type list" fs ts arbitrary: and vs nvs s r 
          rule: typecheck_typecheck_fs.inducts)
   case (tc_app e\<^sub>1 t\<^sub>1 t\<^sub>2 e\<^sub>2)
     thus ?case
@@ -220,10 +197,10 @@ theorem progress: "[] \<turnstile> e : t \<Longrightarrow> is_value e \<or> (\<e
     thus ?case 
       proof (cases "is_value_f fs")
       case False
-        then obtain vs l nvs s e where X: "unfold (Rec fs) = (SRec vs l nvs # s, e)" 
+        then obtain vs nvs s e where X: "unfold (Rec fs) = (SRec vs nvs # s, e)" 
           by (cases "unfold_f fs") simp_all
         with False tc_rec obtain e' where "e \<leadsto>\<^sub>\<beta> e'" by (cases "unfold_f fs") fastforce+
-        with X have "Rec fs \<leadsto> fold (SRec vs l nvs # s) e'" using ev_stack by fastforce
+        with X have "Rec fs \<leadsto> fold (SRec vs nvs # s) e'" using ev_stack by fastforce
         thus ?thesis by fastforce
       qed simp_all
   next case (tc_proj e ts l t)
@@ -232,7 +209,7 @@ theorem progress: "[] \<turnstile> e : t \<Longrightarrow> is_value e \<or> (\<e
       case True
         with tc_proj obtain fs where E: "e = Rec fs \<and> is_value_f fs \<and> [] \<turnstile>\<^sub>f fs : ts" by fastforce
         hence X: "unfold (Proj (Rec fs) l) = ([], Proj (Rec fs) l)" by simp
-        from tc_proj E obtain e' where "lookup_assoc l fs = Some e'" by fastforce
+        from tc_proj E obtain e' where "lookup l fs = Some e'" by fastforce
         with E have "Proj (Rec fs) l \<leadsto>\<^sub>\<beta> e'" by simp
         with X E show ?thesis using ev_stack by fastforce
       next case False
@@ -249,17 +226,11 @@ theorem progress: "[] \<turnstile> e : t \<Longrightarrow> is_value e \<or> (\<e
       qed fastforce+
   qed simp_all
 
-lemma [simp]: "\<Gamma> \<turnstile>\<^sub>f fs : ts \<Longrightarrow> keys ts = keys fs"
-  by (induction \<Gamma> fs ts rule: typecheck_typecheck_fs.inducts(2)) simp_all
-
 lemma [simp]: "\<Gamma> \<turnstile> e : t \<Longrightarrow> unfold e = (s, e') \<Longrightarrow> \<exists>t'. (\<Gamma> \<turnstile> s : t' \<rightarrow> t) \<and> (\<Gamma> \<turnstile> e' : t')"
-  and [simp]: "\<Gamma> \<turnstile>\<^sub>f fs : ts \<Longrightarrow> \<not> is_value_f fs \<Longrightarrow> unfold_f fs = (vs, l, nvs, s, e') \<Longrightarrow> 
-    \<exists>t t' vts nvts. lookup_assoc l ts = Some t \<and> ts = vts @ [(l, t)] @ nvts \<and> 
-      keys vs \<inter> keys nvs = {} \<and> l \<notin> keys vs \<and> l \<notin> keys nvs \<and> 
-        keys fs = insert l (keys vs \<union> keys nvs) \<and> (\<Gamma> \<turnstile> s : t' \<rightarrow> t) \<and> (\<Gamma> \<turnstile> e' : t') \<and> 
-          (\<Gamma> \<turnstile>\<^sub>f vs : vts) \<and> (\<Gamma> \<turnstile>\<^sub>f nvs : nvts)"
-  proof (induction \<Gamma> e t and \<Gamma> fs ts arbitrary: s and vs l nvs s 
-         rule: typecheck_typecheck_fs.inducts)
+  and [simp]: "\<Gamma> \<turnstile>\<^sub>f fs : ts \<Longrightarrow> \<not> is_value_f fs \<Longrightarrow> unfold_f fs = (vs, nvs, s, e') \<Longrightarrow> 
+    \<exists>t t' vts nvts. ts = vts @ [t] @ nvts \<and> (\<Gamma> \<turnstile> s : t' \<rightarrow> t) \<and> (\<Gamma> \<turnstile> e' : t') \<and> (\<Gamma> \<turnstile>\<^sub>f vs : vts) \<and> 
+      (\<Gamma> \<turnstile>\<^sub>f nvs : nvts)"
+  proof (induction \<Gamma> e t and \<Gamma> fs ts arbitrary: s and vs nvs s rule: typecheck_typecheck_fs.inducts)
   case (tc_var x \<Gamma> t)
     moreover hence "\<Gamma> \<turnstile> Var x : t" by auto
     ultimately show ?case by force
@@ -298,12 +269,11 @@ lemma [simp]: "\<Gamma> \<turnstile> e : t \<Longrightarrow> unfold e = (s, e') 
         moreover from tc_rec True have "\<Gamma> \<turnstile> e' : Record ts" by fastforce
         ultimately show ?thesis by blast
       next case False
-        then obtain vs l nvs ss ee' where F: "unfold_f fs = (vs, l, nvs, ss, ee')" 
+        then obtain vs nvs ss ee' where F: "unfold_f fs = (vs, nvs, ss, ee')" 
           by (cases "unfold_f fs") simp_all
-        with tc_rec False obtain t t' vts nvts where T: "lookup_assoc l ts = Some t \<and> 
-          ts = vts @ [(l, t)] @ nvts \<and> keys vs \<inter> keys nvs = {} \<and> l \<notin> keys vs \<and> l \<notin> keys nvs \<and> 
+        with tc_rec False obtain t t' vts nvts where T: "ts = vts @ [t] @ nvts \<and> 
             (\<Gamma> \<turnstile> ss : t' \<rightarrow> t) \<and> (\<Gamma> \<turnstile> e' : t') \<and> (\<Gamma> \<turnstile>\<^sub>f vs : vts) \<and> \<Gamma> \<turnstile>\<^sub>f nvs : nvts" by fastforce
-        hence "\<Gamma> \<turnstile> SRec vs l nvs # ss : t' \<rightarrow> Record ts" using tc_srec by fastforce
+        hence "\<Gamma> \<turnstile> SRec vs nvs # ss : t' \<rightarrow> Record ts" using tc_srec by fastforce
         with tc_rec False F T show ?thesis by fastforce
       qed
   next case (tc_proj \<Gamma> e ts l t)
@@ -321,51 +291,39 @@ lemma [simp]: "\<Gamma> \<turnstile> e : t \<Longrightarrow> unfold e = (s, e') 
         moreover with tc_proj have "\<Gamma> \<turnstile> SProj l # ss : t' \<rightarrow> t" by fastforce
         ultimately show ?thesis by fastforce
       qed
-  next case (tcf_cons \<Gamma> e tt fs ts l')
+  next case (tcf_cons \<Gamma> e tt fs ts)
     thus ?case
       proof (cases "is_value e")
       case True
-        with tcf_cons obtain vs' where V: "unfold_f fs = (vs', l, nvs, s, e') \<and> vs = (l', e) # vs'" 
+        with tcf_cons obtain vs' where V: "unfold_f fs = (vs', nvs, s, e') \<and> vs = e # vs'" 
           by (cases "unfold_f fs") fastforce+
-        moreover with tcf_cons True obtain t t' vts nvts where T: "lookup_assoc l ts = Some t \<and> 
-          ts = vts @ [(l, t)] @ nvts \<and> keys vs' \<inter> keys nvs = {} \<and> l \<notin> keys vs' \<and> l \<notin> keys nvs \<and> 
-            keys fs = insert l (keys vs' \<union> keys nvs) \<and> (\<Gamma> \<turnstile> s : t' \<rightarrow> t) \<and> (\<Gamma> \<turnstile> e' : t') \<and> 
-              (\<Gamma> \<turnstile>\<^sub>f vs' : vts) \<and> \<Gamma> \<turnstile>\<^sub>f nvs : nvts" by fastforce
-        moreover from tcf_cons T have "lookup_assoc l ((l', tt) # ts) = Some t" by auto
-        moreover from tcf_cons V T have "keys vs \<inter> keys nvs = {}" by simp
-        moreover from tcf_cons V T have "l \<notin> keys vs" by auto
-        moreover from V T have "keys ((l', e) # fs) = insert l (keys vs \<union> keys nvs)" by auto
-        moreover from tcf_cons V T have "\<Gamma> \<turnstile>\<^sub>f vs : (l', tt) # vts" by simp
-        ultimately show ?thesis by auto
-      qed fastforce+
+        moreover with tcf_cons True obtain t t' vts nvts where T: "ts = vts @ [t] @ nvts \<and> 
+          (\<Gamma> \<turnstile> s : t' \<rightarrow> t) \<and> (\<Gamma> \<turnstile> e' : t') \<and> (\<Gamma> \<turnstile>\<^sub>f vs' : vts) \<and> \<Gamma> \<turnstile>\<^sub>f nvs : nvts" by fastforce
+        moreover hence "tt # ts = (tt # vts) @ [t] @ nvts" by simp
+        moreover from tcf_cons V T have "\<Gamma> \<turnstile>\<^sub>f vs : tt # vts" by simp
+        ultimately show ?thesis by blast
+      next case False
+        with tcf_cons obtain t' where "(\<Gamma> \<turnstile> s : t' \<rightarrow> tt) \<and> \<Gamma> \<turnstile> e' : t'" by fastforce
+        moreover from tcf_cons False have "\<Gamma> \<turnstile>\<^sub>f vs : []" by simp
+        moreover from tcf_cons False have "\<Gamma> \<turnstile>\<^sub>f nvs : ts" by simp
+        ultimately show ?thesis by fastforce
+      qed
   qed simp_all
 
-lemma "\<Gamma> \<turnstile> e : t \<Longrightarrow> True"
-  and [simp]: "\<Gamma> \<turnstile>\<^sub>f vs : vts \<Longrightarrow> \<Gamma> \<turnstile>\<^sub>f nvs : nvts \<Longrightarrow> keys vs \<inter> keys nvs = {} \<Longrightarrow> 
-    \<Gamma> \<turnstile>\<^sub>f vs @ nvs : vts @ nvts"
-  proof (induction \<Gamma> e t and \<Gamma> vs vts rule: typecheck_typecheck_fs.inducts) 
-  case (tcf_cons \<Gamma> e t fs ts l)
-    hence "l \<notin> keys (fs @ nvs)" by auto
-    with tcf_cons show ?case by simp
-  qed simp_all
+lemma [simp]: "\<Gamma> \<turnstile>\<^sub>f vs : vts \<Longrightarrow> \<Gamma> \<turnstile>\<^sub>f nvs : nvts \<Longrightarrow> \<Gamma> \<turnstile>\<^sub>f vs @ nvs : vts @ nvts"
+  by (induction \<Gamma> vs vts rule: typecheck_typecheck_fs.inducts(2)) simp_all
 
 lemma [simp]: "\<Gamma> \<turnstile> s : t' \<rightarrow> t \<Longrightarrow> \<Gamma> \<turnstile> e : t' \<Longrightarrow> \<Gamma> \<turnstile> fold s e : t"
   by (induction \<Gamma> s t' t rule: typecheck_stack.induct) simp_all
 
-lemma [simp]: "keys (incr_fs x fs) = keys fs"
-  by (induction x fs rule: incr_incr_fs.induct(2)) simp_all
-
 lemma [simp]: "\<Gamma> \<turnstile> e : t \<Longrightarrow> x \<le> length \<Gamma> \<Longrightarrow> insert_at x t' \<Gamma> \<turnstile> incr x e : t"
-  and [simp]: "\<Gamma> \<turnstile>\<^sub>f fs : ts \<Longrightarrow> x \<le> length \<Gamma> \<Longrightarrow> insert_at x t' \<Gamma> \<turnstile>\<^sub>f incr_fs x fs : ts"
+  and [simp]: "\<Gamma> \<turnstile>\<^sub>f fs : ts \<Longrightarrow> x \<le> length \<Gamma> \<Longrightarrow> insert_at x t' \<Gamma> \<turnstile>\<^sub>f map (incr x) fs : ts"
   by (induction \<Gamma> e t and \<Gamma> fs ts arbitrary: x and x rule: typecheck_typecheck_fs.inducts) 
      fastforce+
 
-lemma [simp]: "keys (subst_fs x e' fs) = keys fs"
-  by (induction x e' fs rule: subst_subst_fs.induct(2)) simp_all
-
 lemma [simp]: "insert_at x t' \<Gamma> \<turnstile> e : t \<Longrightarrow> x \<le> length \<Gamma> \<Longrightarrow> \<Gamma> \<turnstile> e' : t' \<Longrightarrow> \<Gamma> \<turnstile> subst x e' e : t"
   and [simp]: "insert_at x t' \<Gamma> \<turnstile>\<^sub>f fs : ts \<Longrightarrow> x \<le> length \<Gamma> \<Longrightarrow> \<Gamma> \<turnstile> e' : t' \<Longrightarrow> 
-    \<Gamma> \<turnstile>\<^sub>f subst_fs x e' fs : ts"
+    \<Gamma> \<turnstile>\<^sub>f map (subst x e') fs : ts"
   proof (induction "insert_at x t' \<Gamma>" e t and "insert_at x t' \<Gamma>" fs ts arbitrary: \<Gamma> x e' and \<Gamma> x e' 
          rule: typecheck_typecheck_fs.inducts)
   case (tc_var y t)
@@ -375,9 +333,8 @@ lemma [simp]: "insert_at x t' \<Gamma> \<turnstile> e : t \<Longrightarrow> x \<
     ultimately show ?case by simp
   qed fastforce+
 
-lemma [elim]: "\<Gamma> \<turnstile>\<^sub>f fs : ts \<Longrightarrow> lookup_assoc l fs = Some e \<Longrightarrow> lookup_assoc l ts = Some t \<Longrightarrow> 
-    \<Gamma> \<turnstile> e : t" 
-  by (induction \<Gamma> fs ts rule: typecheck_typecheck_fs.inducts(2)) (simp, simp_all split: if_splits)
+lemma [elim]: "\<Gamma> \<turnstile>\<^sub>f fs : ts \<Longrightarrow> lookup l fs = Some e \<Longrightarrow> lookup l ts = Some t \<Longrightarrow> \<Gamma> \<turnstile> e : t" 
+  by (induction l fs arbitrary: ts rule: lookup.induct) auto
 
 lemma preservation\<^sub>\<beta>: "e \<leadsto>\<^sub>\<beta> e' \<Longrightarrow> \<Gamma> \<turnstile> e : t \<Longrightarrow> \<Gamma> \<turnstile> e' : t"
   by (induction e e' rule: reduce.induct) fastforce+
